***NO_CI*** wip with Aseem; adding support for user tactics interpreted on the normalizer

src/tactics/FStar.Tactics.Basic.fs
@@ -179,7 +179,7 @@ let with_cur_goal (nm:string) (f:goal -> tac<'a>) : tac<'a>
         | [] -> fail "No more goals"
         | hd::tl -> f hd))
 
-let smt : tac<unit> = 
+let smt : tac<unit> =
     with_cur_goal "smt" (fun g ->
     bind dismiss (fun _ ->
     bind (add_goals [({g with goal_ty=U.t_true})]) (fun _ ->
@@ -292,14 +292,13 @@ let seq (t1:tac<unit>)
 //Q: should it instead be
 //    val forall_intro_squash_gtot_join  : #a:Type -> #p:(a -> GTot Type) -> $f:(x:a -> GTot (squash (p x))) -> Tot (forall (x:a). p x)
 //   ?? Note the additional squash on f
-let intros : tac<(list<name>)>
+let intros : tac<binders>
    = with_cur_goal "intros" (fun goal ->
          match U.destruct_typ_as_formula goal.goal_ty with
          | Some (U.QAll(bs, pats, body)) ->
            //TODO!
            //ignoring the qualifiers on bs and the pats for now
            //need to restore that!
-           let names = List.map fst bs in
            let new_context = Env.push_binders goal.context bs in
            let new_goal = {
              context=new_context;
@@ -311,7 +310,7 @@ let intros : tac<(list<name>)>
 //                    (Print.term_to_string body);
            bind dismiss (fun _ ->
            bind (add_goals [new_goal]) (fun _ ->
-           ret names))
+           ret bs))
          | _ ->
            fail "Cannot intro this goal, expected a forall")
 
@@ -438,6 +437,29 @@ let clear_hd (x:name) : tac<unit>
                     bind dismiss (fun _ ->
                     add_goals [new_goal]))
 
+let revert : tac<unit>
+    = with_cur_goal "revert" (fun goal ->
+      match Env.pop_bv goal.context with
+      | None -> fail "Cannot clear_hd; empty context"
+      | Some (x, env') ->
+        let fns = FStar.Syntax.Free.names goal.goal_ty in
+        if not (Util.set_mem x fns)
+        then clear_hd x
+        else let new_goal =
+            match un_squash x.sort, un_squash goal.goal_ty with
+            | Some p, Some q ->
+                { goal with
+                context = env';
+                goal_ty = U.mk_imp p q
+                }
+            | _ ->
+                { goal with
+                context = env';
+                goal_ty = U.mk_forall x goal.goal_ty
+                } in
+        bind dismiss (fun _ ->
+        add_goals [new_goal]))
+
 let revert_hd (x:name) : tac<unit>
     = with_cur_goal "revert_hd" (fun goal ->
       match Env.pop_bv goal.context with
@@ -523,16 +545,16 @@ let merge_sub_goals : tac<unit> =
          let goals = p.goals |> List.map (fun x -> Print.term_to_string x.goal_ty) |> String.concat "\n\t" in
          fail (BU.format1 "Cannot merge sub-goals: not enough sub-goals\n\tGoals are: %s" goals)))
 
-let rec visit_strengthen (try_strengthen:tac<unit>)
+let rec visit (callback:tac<unit>)
     : tac<unit>
     = focus_cur_goal "visit_strengthen"
-        (or_else try_strengthen
+        (or_else callback
                 (with_cur_goal "visit_strengthen_else" (fun goal ->
                     match U.destruct_typ_as_formula goal.goal_ty with
                     | None -> begin
                       match (SS.compress goal.goal_ty).n with
                       | Tm_meta _ ->
-                        map_meta (visit_strengthen try_strengthen)
+                        map_meta (visit callback)
                       | _ ->
                         printfn "Not a formula, split to smt %s" (Print.term_to_string goal.goal_ty);
                         smt
@@ -543,24 +565,234 @@ let rec visit_strengthen (try_strengthen:tac<unit>)
                         ret ()
 
                     | Some (U.QAll(xs, _, _)) ->
-                      bind intros (fun names ->
+                      bind intros (fun binders ->
                       //printfn "At forall %s" (List.map Print.bv_to_string names |> String.concat ", ");
-                      bind (visit_strengthen try_strengthen) (fun _ ->
-                           (revert_all_hd names)))
+                      bind (visit callback) (fun _ ->
+                           (revert_all_hd (List.map fst binders))))
 
                     | Some (U.BaseConn(l, _))
                         when Ident.lid_equals l SC.and_lid ->
-                      bind (seq split (visit_strengthen try_strengthen)) (fun _ ->
+                      bind (seq split (visit callback)) (fun _ ->
                             merge_sub_goals)
 
                     | Some (U.BaseConn(l, _))
                         when Ident.lid_equals l SC.imp_lid ->
                       bind imp_intro (fun h ->
-                      bind (visit_strengthen try_strengthen) (fun _ ->
+                      bind (visit callback) (fun _ ->
                       revert_hd h))
 
                     | Some (U.BaseConn(l, _)) ->
                       or_else trivial smt)))
+
+let fstar_tactics_lid s = Ident.lid_of_path (["FStar"; "Tactics"]@[s]) Range.dummyRange
+let by_tactic_lid = fstar_tactics_lid "by_tactic"
+let lid_as_tm l = S.lid_as_fv l Delta_constant None |> S.fv_to_tm
+let mk_tactic_lid_as_term (s:string) = lid_as_tm (fstar_tactics_lid s)
+let fstar_tactics_term   = mk_tactic_lid_as_term "term"
+let fstar_tactics_env    = mk_tactic_lid_as_term "env"
+let fstar_tactics_binder = mk_tactic_lid_as_term "binder"
+let fstar_tactics_binders= mk_tactic_lid_as_term "binders"
+let fstar_tactics_goal   = mk_tactic_lid_as_term "goal"
+let fstar_tactics_goals  = mk_tactic_lid_as_term "goals"
+let fstar_tactics_Failed = S.fv_to_tm (S.lid_as_fv (fstar_tactics_lid "Failed") Delta_constant (Some Data_ctor))
+let fstar_tactics_Success= S.fv_to_tm (S.lid_as_fv (fstar_tactics_lid "Success") Delta_constant (Some Data_ctor))
+let lid_Mktuple2 = U.mk_tuple_data_lid 2 Range.dummyRange
+
+let embed_binder (b:binder) : term = S.bv_to_name (fst b)
+let unembed_binder (t:term) : binder =
+    let t = U.unascribe t in
+    match t.n with
+    | Tm_name bv -> S.mk_binder bv
+    | _ -> failwith "Not an embedded binder"
+
+let embed_pair (x:('a * 'b)) (embed_a:'a -> term) (t_a:term) (embed_b:'b -> term) (t_b:term) : term =
+    S.mk_Tm_app (S.mk_Tm_uinst (lid_as_tm lid_Mktuple2) [U_zero;U_zero])
+                [S.iarg t_a;
+                 S.iarg t_b;
+                 S.as_arg (embed_a (fst x));
+                 S.as_arg (embed_b (snd x))]
+                None
+                Range.dummyRange
+
+let unembed_pair (pair:term) (unembed_a:term -> 'a) (unembed_b:term -> 'b) : ('a * 'b) =
+    let pairs = U.unascribe pair in
+    let hd, args = U.head_and_args pair in
+    match (U.un_uinst hd).n, args with
+    | Tm_fvar fv, [_; _; (a, _); (b, _)] when S.fv_eq_lid fv lid_Mktuple2 ->
+      unembed_a a, unembed_b b
+    | _ -> failwith "Not an embedded pair"
+
+
+let rec embed_list (l:list<'a>) (embed_a: ('a -> term)) (t_a:term) : term =
+    match l with
+    | [] -> S.mk_Tm_app (S.mk_Tm_uinst (lid_as_tm FStar.Syntax.Const.nil_lid) [U_zero])
+                        [S.iarg t_a]
+                        None
+                        Range.dummyRange
+    | hd::tl ->
+            S.mk_Tm_app (S.mk_Tm_uinst (lid_as_tm FStar.Syntax.Const.cons_lid) [U_zero])
+                        [S.iarg t_a;
+                         S.as_arg (embed_a hd);
+                         S.as_arg (embed_list tl embed_a t_a)]
+                        None
+                        Range.dummyRange
+
+let rec unembed_list (l:term) (unembed_a: (term -> 'a)) : list<'a> =
+    let l = U.unascribe l in
+    let hd, args = U.head_and_args l in
+    match (U.un_uinst hd).n, args with
+    | Tm_fvar fv, _
+        when S.fv_eq_lid fv SC.nil_lid -> []
+
+    | Tm_fvar fv, [_t; (hd, _); (tl, _)]
+        when S.fv_eq_lid fv SC.cons_lid ->
+      unembed_a hd :: unembed_list tl unembed_a
+
+    | _ ->
+      failwith (BU.format1 "Not an embedded list: %s" (Print.term_to_string l))
+
+let embed_binders l = embed_list l embed_binder fstar_tactics_binder
+let unembed_binders t = unembed_list t unembed_binder
+
+let embed_env (env:Env.env) : term = embed_list (Env.all_binders env) embed_binder fstar_tactics_binder
+
+let unembed_env (env:Env.env) (embedded_env:term) : Env.env =
+    let binders = unembed_list embedded_env unembed_binder in
+    Env.push_binders env binders
+
+let embed_goal (g:goal) : term =
+    embed_pair (g.context, g.goal_ty) embed_env fstar_tactics_env (fun x -> x) fstar_tactics_term
+
+let unembed_goal (env:Env.env) (t:term) : goal =
+    let env, goal_ty = unembed_pair t (unembed_env env) (fun x -> x) in
+    {
+      context = env;
+      goal_ty = goal_ty;
+      witness = None //TODO: sort this out for proof-relevant goals
+    }
+
+let embed_goals (l:list<goal>) : term = embed_list l embed_goal fstar_tactics_goal
+let unembed_goals (env:Env.env) (egs:term) : list<goal> = unembed_list egs (unembed_goal env)
+
+type state = list<goal> * list<goal>
+
+let embed_state (s:state) : term =
+    embed_pair s embed_goals fstar_tactics_goals embed_goals fstar_tactics_goals
+
+let unembed_state (env:Env.env) (s:term) : state =
+    let s = U.unascribe s in
+    unembed_pair s (unembed_goals env) (unembed_goals env)
+
+let embed_unit (u:unit) : term = SC.exp_unit
+let unembed_unit (_:term) :unit = ()
+
+let embed_string (s:string) : term =
+    let bytes = BU.unicode_of_string s in
+    S.mk (Tm_constant(FStar.Const.Const_string(bytes, Range.dummyRange)))
+         None
+         Range.dummyRange
+
+let unembed_string (t:term) : string =
+    let t = U.unascribe t in
+    match t.n with
+    | Tm_constant(FStar.Const.Const_string(bytes, _)) ->
+      BU.string_of_unicode bytes
+    | _ ->
+      failwith "Not an embedded string"
+
+let embed_result (res:result<'a>) (embed_a:'a -> term) (t_a:typ) : term =
+    match res with
+    | Failed (msg, ps) ->
+      S.mk_Tm_app (S.mk_Tm_uinst fstar_tactics_Failed [U_zero])
+                  [S.iarg t_a;
+                   S.as_arg (embed_string msg);
+                   S.as_arg (embed_state (ps.goals, ps.smt_goals))]
+                  None
+                  Range.dummyRange
+    | Success (a, ps) ->
+      S.mk_Tm_app (S.mk_Tm_uinst fstar_tactics_Success [U_zero])
+                  [S.iarg t_a;
+                   S.as_arg (embed_a a);
+                   S.as_arg (embed_state (ps.goals, ps.smt_goals))]
+                  None
+                  Range.dummyRange
+
+let unembed_result (env:Env.env) (res:term) : either<state, (string * state)> =
+    let res = U.unascribe res in
+    let hd, args = U.head_and_args res in
+    match (U.un_uinst hd).n, args with
+    | Tm_fvar fv, [_t; _unit; (embedded_state, _)]
+        when S.fv_eq_lid fv (fstar_tactics_lid "Success") ->
+      Inl (unembed_state env embedded_state)
+
+    | Tm_fvar fv, [_t; (embedded_string, _); (embedded_state, _)]
+        when S.fv_eq_lid fv (fstar_tactics_lid "Failed") ->
+      Inr (unembed_string embedded_string, unembed_state env embedded_state)
+
+    | _ -> failwith (BU.format1 "Not an embedded result: %s" (Print.term_to_string res))
+
+let mk_tactic_interpretation (ps:proofstate) (env:Env.env) (t:tac<'a>) (embed_a:'a -> term) (t_a:typ) (args:args) : term =
+ (*  We have: t () embedded_state
+     The idea is to:
+        1. unembed the state
+        2. run the `t` tactic
+        3. embed the result and final state and return it to the normalizer
+  *)
+  match args with
+  | [_unit; (embedded_state, _)] ->
+    printfn "Reached forall_intro_interpretation, goals are: %s" (Print.term_to_string embedded_state);
+    let goals, smt_goals = unembed_state env embedded_state in
+    let ps = {ps with goals=goals; smt_goals=smt_goals} in
+    let res = run t ps in
+    embed_result res embed_a t_a
+  | _ ->
+    failwith ("Unexpected application of 'forall_intro'")
+
+let primitive_steps ps env : list<N.primitive_step> =
+    [{N.name=fstar_tactics_lid "forall_intros";
+      N.arity=2;
+      N.interpretation=mk_tactic_interpretation ps env intros embed_binders fstar_tactics_binders};
+
+     {N.name=fstar_tactics_lid "smt";
+      N.arity=2;
+      N.interpretation=mk_tactic_interpretation ps env smt embed_unit FStar.TypeChecker.Common.t_unit};
+
+     {N.name=fstar_tactics_lid "revert";
+      N.arity=2;
+      N.interpretation=mk_tactic_interpretation ps env revert embed_unit FStar.TypeChecker.Common.t_unit}]
+
+let evaluate_user_tactic : tac<unit>
+    = with_cur_goal "evaluate_user_tactic" (fun goal ->
+      bind get (fun proof_state ->
+          let hd, args = U.head_and_args goal.goal_ty in
+          match (U.un_uinst hd).n, args with
+          | Tm_fvar fv, [(tactic, _); (assertion, _)]
+                when S.fv_eq_lid fv by_tactic_lid ->
+            (* We're making (reify (tactic ()) [(goal)] *)
+            let tm = S.mk_Tm_app (U.mk_reify (S.mk_Tm_app tactic [S.as_arg SC.exp_unit] None Range.dummyRange))
+                                 [S.as_arg (embed_state ([{goal with goal_ty=assertion}], []))]
+                                 None
+                                 Range.dummyRange in
+            let steps = [N.Reify; N.Beta; N.UnfoldUntil Delta_constant; N.Zeta; N.Iota; N.Primops] in
+            printfn "Starting normalizer with %s" (Print.term_to_string tm);
+            Options.set_option "debug_level" (Options.List [Options.String "Norm"]);
+            let result = N.normalize_with_primitive_steps (primitive_steps proof_state goal.context) steps goal.context tm in
+            Options.set_option "debug_level" (Options.List []);
+            printfn "Reduced tactic: got %s" (Print.term_to_string result);
+            begin match unembed_result goal.context result with
+                | Inl (goals, smt_goals) ->
+                  bind dismiss (fun _ ->
+                  bind (add_goals goals) (fun _ ->
+                  add_smt_goals smt_goals))
+
+                | Inr (msg, (goals, smt_goals)) ->
+                  bind dismiss (fun _ ->
+                  bind (add_goals goals) (fun _ ->
+                  bind (add_smt_goals smt_goals) (fun _ ->
+                  fail msg)))
+            end
+          | _ ->
+            fail "Not a user tactic"))
 
 let rec simplify_eq_impl : tac<unit>
     = with_cur_goal "simplify_eq_impl" (fun goal ->
@@ -576,7 +808,7 @@ let rec simplify_eq_impl : tac<unit>
                  //clear_hd: get rid of the eq_h in the context
                  //we're left with rhs[e/x]
             bind (clear_hd eq_h) (fun _ ->
-            visit_strengthen simplify_eq_impl))))
+            visit simplify_eq_impl))))
           | _ ->
             printfn "%s is not an equality imp" (Print.term_to_string goal.goal_ty);
             fail "Not an equality implication")
@@ -605,11 +837,12 @@ let preprocess (env:Env.env) (goal:term) : list<(Env.env * term)> =
     then [env, goal]
     else let _ = printfn "About to preprocess %s\n" (Print.term_to_string goal) in
          let p = proofstate_of_goal_ty env goal in
-         match run (visit_strengthen simplify_eq_impl) p with
+         match run (visit evaluate_user_tactic) p with
          | Success (_, p2) ->
            (p2.goals @ p2.smt_goals) |> List.map (fun g ->
              printfn "Got goal: %s" (Print.term_to_string g.goal_ty);
              g.context, g.goal_ty)
          | Failed (msg, _) ->
            printfn "Tactic failed: %s" msg;
+           printfn "Got goal: %s" (Print.term_to_string goal);
            [env, goal]
