src/typechecker/FStar.TypeChecker.Normalize.fsi
@@ -41,7 +41,11 @@ type step =
   | CompressUvars
   | NoFullNorm
 and steps = list<step>
-
+type primitive_step = {
+    name:FStar.Ident.lid;
+    arity:int;
+    interpretation:(args -> term)
+}
 val eta_expand_with_type :term -> typ -> term
 val eta_expand:           Env.env -> term -> term
 val comp_to_comp_typ:     Env.env -> comp -> comp_typ
@@ -52,6 +56,6 @@ val normalize_comp:       steps -> Env.env -> comp -> comp
 val normalize_refinement: steps -> Env.env -> typ -> typ
 val ghost_to_pure:        Env.env -> comp -> comp
 val ghost_to_pure_lcomp:  Env.env -> lcomp -> lcomp
-
+val normalize_with_primitive_steps : list<primitive_step> -> list<step> -> Env.env -> term -> term
 val term_to_string:  Env.env -> term -> string
 val comp_to_string:  Env.env -> comp -> string
