examples/tactics/micro-benchmarks/UserTactics.Example1.fst
@@ -1,10 +1,11 @@
 module UserTactics.Example1 
 open FStar.Tactics
-   
+
+#set-options "--lax"
 (* -------------------------------------------------------------------------------- *)
 let cur_goal () : Tac goal = 
   let goals = TAC?.get () in 
-  match goals with 
+  match fst goals with 
   | [] -> fail #goal "No more goals"
   | hd::_ -> hd
 
@@ -17,9 +18,9 @@ let destruct_equality_implication (t:term) : option (formula * term) =
      | _ -> None)
   | _ -> None
     
-let rec simplify_eq_implication () 
-  : Tac unit
-  = let context, goal_t = cur_goal () in 
+let rec simplify_eq_implication : tactic
+  = fun () -> 
+    let context, goal_t = cur_goal () in 
     match destruct_equality_implication goal_t with
     | None -> fail "Not an equality implication"
     | Some (_, rhs) ->
@@ -30,7 +31,15 @@ let rec simplify_eq_implication ()
 
 ////////////////////////////////////////////////////////////////////////////////
 
+let rec just_do_intros : tactic = fun () ->
+  let _ = forall_intros () in
+  let _ = smt () in
+  revert ()
 
-let test_1 = assert_by_tactic simplify_eq_implication 
-                             (forall (x:int). x==0 ==> (forall (y:int). y==0 ==> x==y))
+#reset-options// "--debug UserTactics.Example1 --debug_level Norm"
+let test_1 = 
+  assert_by_tactic just_do_intros
+                   (forall (x:int). x==0 ==> (forall (y:int). y==0 ==> x==y));
+  assert_by_tactic just_do_intros
+                   (forall (y:int). y==0 ==> 0==y)
 
