ulib/FStar.All.fst
@@ -31,7 +31,7 @@ sub_effect EXN ~> ALL { lift_wp = lift_exn_all }
 
 effect All (a:Type) (pre:all_pre) (post:(heap -> Tot (all_post a))) =
   ALL a
-    (fun (p : all_post a) (h : heap) -> pre h /\ (forall ra h1. pre h /\ post h ra h1 ==> p ra h1))
+    (fun (p : all_post a) (h : heap) -> pre h /\ (forall ra h1. post h ra h1 ==> p ra h1))
 effect ML (a:Type) = ALL a (all_null_wp heap a)
 
 assume val pipe_right : 'a -> ('a -> ML 'b) -> ML 'b
